sympy/tensor/functions.lean
@@ -1,6 +1,13 @@
 import sympy.tensor.tensor
 import sympy.vector.functions
-open Tensor
+import Lemma.Algebra.LengthInsertIdx.eq.Add1Length.of.Le_Length
+import Lemma.Algebra.LengthEraseIdx.eq.SubLength_1.of.Lt_Length
+import Lemma.Algebra.EqAdd_Sub.of.Ge
+import Lemma.Logic.EqUFnS.of.Eq
+import Lemma.Algebra.Set.eq.AppendTake__Cons_Drop.of.Lt_Length
+import Lemma.List.TakeInsertIdx.eq.Take.of.Ge
+import Lemma.List.TakeEraseIdx.eq.Take.of.Ge
+open Tensor Algebra Logic List
 
 /--
 [exp](https://pytorch.org/docs/stable/generated/torch.exp.html)
@@ -18,3 +25,35 @@ instance [Exp α] : Exp (Tensor α s) where
 -/
 instance [Log α] : Log (Tensor α s) where
   log X := ⟨Log.log X.data⟩
+
+
+/--
+[softmax](https://pytorch.org/docs/stable/generated/torch.softmax.html)
+-/
+def Tensor.softmax [Zero α] [Div α] [Exp α] (x : Tensor α s) (dim : ℕ := s.length - 1) : Tensor α s :=
+  let x_exp := exp x
+  let x_sum : Tensor α s :=
+    if h : dim < s.length then
+      let x_sum := x_exp.sum dim
+      let x_sum := x_sum.unsqueeze dim
+      have h_dim : dim < ((s.eraseIdx dim).insertIdx dim 1).length := by
+        rw [LengthInsertIdx.eq.Add1Length.of.Le_Length] <;>
+          rw [LengthEraseIdx.eq.SubLength_1.of.Lt_Length h]
+        .
+          rwa [EqAdd_Sub.of.Ge]
+          apply Ge_1.of.Gt h
+        .
+          apply Le_Sub_1.of.Lt h
+      let x_sum := x_sum.repeat s[dim] ⟨dim, h_dim⟩
+      cast
+        (by
+          apply EqUFnS.of.Eq
+          rw [Set.eq.AppendTake__Cons_Drop.of.Lt_Length (by simp [h_dim])]
+          rw [TakeInsertIdx.eq.Take.of.Ge (by simp)]
+          rw [TakeEraseIdx.eq.Take.of.Ge (by simp)]
+          sorry
+        )
+        x_sum
+    else
+      x_exp
+  x_exp / x_sum
