Lemma/List/EqInsertIdx/of/Gt_Length.lean
@@ -1,0 +1,16 @@
+import sympy.Basic
+
+
+@[main]
+private lemma main
+  {a : List α}
+-- given
+  (h : i > a.length)
+  (x : α) :
+-- imply
+  a.insertIdx i x = a :=
+-- proof
+  List.insertIdx_of_length_lt h
+
+
+-- created on 2025-10-03
