Lemma/List/EraseIdx/eq/Append_Drop_Add_1.lean
@@ -1,0 +1,15 @@
+import sympy.Basic
+
+
+@[main]
+private lemma main
+-- given
+  (l : List α)
+  (i : ℕ) :
+-- imply
+  l.eraseIdx i = l.take i ++ l.drop (i + 1) :=
+-- proof
+  List.eraseIdx_eq_take_drop_succ l i
+
+
+-- created on 2025-10-03
