Lemma/List/InsertIdx/eq/Append_InsertIdxDrop/of/Ge/Le_Length.lean
@@ -1,0 +1,35 @@
+import Lemma.Algebra.Gt.is.Ge.Ne
+import Lemma.List.InsertIdx.eq.Append_InsertIdxDrop.of.Gt
+import Lemma.Algebra.EqAppendTake__Drop
+import Lemma.Algebra.InsertIdxAppend.eq.Append_InsertIdx.of.Le_Length
+import Lemma.Algebra.LengthTake.eq.Min_Length
+import Lemma.Algebra.EqMin.of.Le
+open Algebra List
+
+
+@[main]
+private lemma main
+  {a : List α}
+-- given
+  (h_i : i ≤ a.length)
+  (h : i ≥ j)
+  (x : α) :
+-- imply
+  a.insertIdx i x = a.take j ++ (a.drop j).insertIdx (i - j) x := by
+-- proof
+  by_cases h_j : i = j
+  ·
+    subst h_j
+    simp
+    conv_lhs =>
+      rw [← EqAppendTake__Drop a i]
+    rw [InsertIdxAppend.eq.Append_InsertIdx.of.Le_Length]
+    <;> rw [LengthTake.eq.Min_Length]
+    <;> rw [EqMin.of.Le h_i]
+    simp
+  ·
+    apply InsertIdx.eq.Append_InsertIdxDrop.of.Gt ∘ Gt.of.Ge.Ne h
+    assumption
+
+
+-- created on 2025-10-03
