Lemma/List/InsertIdx/eq/Append_InsertIdxDrop/of/Gt.lean
@@ -1,0 +1,46 @@
+import Lemma.Algebra.EqAppendTake__Drop
+import Lemma.Algebra.InsertIdxAppend.eq.Append_InsertIdx.of.Le_Length
+import Lemma.Algebra.LengthTake.eq.Min_Length
+import Lemma.Algebra.EqMin.of.Le
+import Lemma.List.EqInsertIdx.of.Gt_Length
+import Lemma.Algebra.EqTake.of.Ge_Length
+import Lemma.Algebra.Drop.eq.Nil.of.Ge_Length
+import Lemma.Algebra.Ge.of.Gt
+import Lemma.Algebra.Gt.of.Gt.Gt
+import Lemma.Algebra.Ge_Min.of.Ge
+open Algebra List
+
+
+@[main]
+private lemma main
+  {a : List α}
+-- given
+  (h : i > j)
+  (x : α) :
+-- imply
+  a.insertIdx i x = a.take j ++ (a.drop j).insertIdx (i - j) x := by
+-- proof
+  by_cases h_j : j ≤ a.length
+  · 
+    conv_lhs =>
+      rw [← EqAppendTake__Drop a j]
+    rw [InsertIdxAppend.eq.Append_InsertIdx.of.Le_Length] <;> 
+      rw [LengthTake.eq.Min_Length]
+    · 
+      rwa [EqMin.of.Le]
+    · 
+      apply Ge_Min.of.Ge ∘ Ge.of.Gt
+      assumption
+  · 
+    simp at h_j
+    have h_i := Gt.of.Gt.Gt h h_j
+    rw [EqInsertIdx.of.Gt_Length h_i]
+    have h_j := Ge.of.Gt h_j
+    rw [EqTake.of.Ge_Length h_j]
+    rw [Drop.eq.Nil.of.Ge_Length h_j]
+    simp
+    have h_ij := Sub.gt.Zero.of.Gt.nat h
+    rw [EqInsertIdx.of.Gt_Length h_ij]
+
+
+-- created on 2025-10-03
