Lemma/List/TakeEraseIdx/eq/Take/of/Ge.lean
@@ -1,0 +1,26 @@
+import Lemma.Algebra.EqTake.of.Ge_Length
+import Lemma.List.EqEraseIdx.of.Ge_Length
+import Lemma.List.EraseIdx.eq.Append_Drop_Add_1
+open Algebra List
+
+
+@[main]
+private lemma main
+-- given
+  (h : i ≥ j)
+  (a : List α) :
+-- imply
+  (a.eraseIdx i).take j = a.take j := by
+-- proof
+  by_cases hlen : j ≤ a.length
+  ·
+    have h_le_length : j ≤ (a.take i).length := by
+      rw [List.length_take]
+      exact le_min h hlen
+    rw [EraseIdx.eq.Append_Drop_Add_1]
+    rw [List.take_append_of_le_length h_le_length, List.take_take, min_eq_left h]
+  ·
+    rw [EqEraseIdx.of.Ge_Length (by linarith)]
+
+
+-- created on 2025-10-03
