Lemma/List/TakeInsertIdx/eq/Take/of/Ge.lean
@@ -1,0 +1,31 @@
+import Lemma.List.InsertIdx.eq.Append_InsertIdxDrop.of.Ge.Le_Length
+import Lemma.List.EqInsertIdx.of.Gt_Length
+import Lemma.Algebra.EqTakeAppend.of.Eq_Length
+import Lemma.Algebra.LengthTake.eq.Min_Length
+import Lemma.Algebra.EqMin.of.Le
+import Lemma.Algebra.Le.of.Le.Le
+open List Algebra
+
+
+@[main]
+private lemma main
+-- given
+  (h : i ≥ j)
+  (a : List α)
+  (x : α) :
+-- imply
+  (a.insertIdx i x).take j = a.take j := by
+-- proof
+  by_cases h_i : i ≤ a.length
+  ·
+    rw [InsertIdx.eq.Append_InsertIdxDrop.of.Ge.Le_Length h_i h]
+    apply EqTakeAppend.of.Eq_Length
+    rw [LengthTake.eq.Min_Length]
+    apply EqMin.of.Le ∘ Le.of.Le.Le h
+    assumption
+  ·
+    rw [EqInsertIdx.of.Gt_Length]
+    linarith
+
+
+-- created on 2025-10-03
