Lemma/Tensor/Softmax/eq/Div_SumExp.lean
@@ -1,0 +1,17 @@
+import sympy.tensor.functions
+import sympy.Basic
+
+
+@[main]
+private lemma main
+  [Exp α] [Zero α] [Div α]
+-- given
+  (x : Tensor α s) :
+-- imply
+  x.softmax = exp x / (exp x).sum := by
+-- proof
+  unfold Tensor.softmax
+  simp
+
+
+-- created on 2025-10-03
